Leader election protocol refresh

examples/Election.v
@@ -2,12 +2,15 @@ From CTree Require Import
   CTree.Core
   Logic.Ctl
   Utils.Vectors
-  Events.WriterE
-  CTree.Logic.Trans
-  CTree.Logic.AF
   CTree.Equ
+  CTree.SBisim
+  CTree.Logic.AG
+  CTree.Logic.AF
+  CTree.Logic.AX
+  CTree.Logic.State
+  CTree.Logic.Bind
   CTree.Events.Writer
-  CTree.Events.Net.
+  CTree.Events.Net.Uniring.
 
 From Coq Require Import
   Fin
@@ -17,7 +20,7 @@ From Coq Require Import
 
 Set Implicit Arguments.
 
-Import ListNotations CTreeNotations CtlNotations MessageOrderScheduler.
+Import ListNotations CTreeNotations CtlNotations.
 Local Close Scope list_scope.
 Local Open Scope ctree_scope.
 Local Open Scope fin_vector_scope.
@@ -29,7 +32,7 @@ Section Election.
     | Candidate (u: fin' n)
     | Elected (u: fin' n).
 
-  Notation netE := (netE n message).
+  Notation netE := (netE message).
 
   Definition msg_id(m: message): fin' n :=
     match m with
@@ -46,17 +49,14 @@ Section Election.
 
   Notation continue := (Ret (inl tt)).
   Notation stop := (Ret (inr tt)).
-
+  
   (* Always terminates, conditional on receiving either:
      1. (Candidate candidate), where candidate = id -- I received my own [id] back 
      2. (Elected leader) -- Someone else was elected [leader]
-
-    If scheduled fairly, either 1, 2 should always eventually happen.
-    Should be WG provable.
-  *)
-  Definition proc(id: fin' n): ctree netE (fin' n) :=
-    let right := cycle id in
-    send right (Candidate id) ;;
+   *)
+  Definition elect(id: fin' n): ctree netE unit :=
+    send (Candidate id) ;;
+    (* Recv loop *)
     Ctree.iter
       (fun _ =>
          m <- recv ;;
@@ -64,34 +64,31 @@ Section Election.
          | Some (Candidate candidate) =>
              match Fin_compare candidate id with (* candidate < id *)
              (* [left] neighbor proposed candidate, support her to [right]. *)
-             | Gt => send right (Candidate candidate) ;; continue
+             | Gt => send (Candidate candidate) ;; continue
              (* [left] neighbor proposed a candidate, do not support her. *)
              | Lt => continue
              (* I am the leader, but only I know. Tell my [right] and return. *)
-             | Eq => send right (Elected id) ;; Ret (inr id)
+             | Eq => send (Elected id) ;; stop
              end
          | Some (Elected leader) =>
              (* I am a follower and know the [leader] *)
-             send right (Elected leader) ;; Ret (inr leader)
-         | None => continue (* Recv loop *)
+             send (Elected leader) ;; stop
+         | None =>  stop (* Recv loop *)
          end) tt.
 
-  (* TODO: Instrumentation of [send] *)
-  Definition instr(i: fin' n)(mail: message) : option (fin' n) := Some i.
-  
-
-  Definition election_interp : ctree (writerE (fin' n)) void :=
-    schedule instr (Vector.map proc (fin_all_v n)).
+  Definition election_proto : ctree (writerE NetObs) void :=
+    uring_sched (Vector.map (fun id => {| mbox := None; proc := elect id |}) (fin_all_v n)).
 
   Lemma election_fair: forall (i: fin' n),
-      <( election_interp, Pure |= AF visW \j, i = j )>.
-  Proof.
+      <( election_proto, Pure |= AF visW {fun obs => obs.(id) = i} )>.
+  Proof with auto with ctl.
     intros.
-    unfold election_interp, schedule.
+    unfold election_proto, uring_sched. 
     unfold Ctree.branch.
     rewrite bind_br.
-    apply af_br.
-    intro j. (* First pick *)
+    cright.
+    apply axl_br; split; [csplit; split; auto with ctl|].
+    intro c. (* Nondeterministic pick *)
     rewrite bind_ret_l.
-    
+  Admitted.    
 End Election.
