theories/CTree/Events/Net/Uniring.v
@@ -1,0 +1,136 @@
+From CTree Require Import
+  Utils.Vectors
+  CTree.Core.
+
+From CTree Require Export
+  CTree.Core
+  Events.Core
+  Events.WriterE.
+
+From ExtLib Require Import
+  Structures.MonadState
+  Data.Monads.StateMonad.
+
+From Equations Require Import Equations.
+
+Import CTreeNotations.
+Local Open Scope ctree_scope.
+Local Open Scope fin_vector_scope.
+
+(*| Message passing in unidirectional ring |*)
+Variant netE(T: Type): Type :=
+  | Recv
+  | Send (msg: T).
+
+Arguments Recv {T}.
+Arguments Send {T}.
+
+#[global] Instance encode_netE{T}: Encode (netE T) :=
+  fun e => match e with
+        | Recv => option T
+        | Send _ => unit
+        end.
+
+Arguments encode_netE {T} /.
+
+Definition send {T}: T -> ctree (netE T) unit :=
+  fun p => Ctree.trigger (Send p).
+
+Definition recv {T}: ctree (netE T) (option T) :=
+  Ctree.trigger (@Recv T).
+
+Definition option_dec{A}(o: option A): {o = None} + {exists v, o = Some v} :=
+  match o with
+  | Some x => right (ex_intro (fun v : A => Some x = Some v) x eq_refl)
+  | None => left eq_refl
+  end.
+                                         
+(* Unidirectional ring scheduler for ctrees, based on message passing.
+   1. Pick non-deterministically an [i: fin n], schedule process [i].
+   2. When [i] sends a message to [j], deliver message and schedule [j] next.
+   3. Repeat (2) forever.
+ *)
+Section UniringMsg.
+  Context {n: nat} {T: Type}.
+
+  Notation netE := (netE T).
+  Record Worker := {
+      mbox: option T;
+      proc: ctree netE unit;
+    }.
+
+  Definition observe_worker (w: Worker): option T * ctree' netE unit :=
+    (w.(mbox), observe w.(proc)).
+
+  (* The Type of network observations *)
+  Record NetObs := {
+      id : fin' n;
+      sent : option T;
+      recd: option T;
+      term: bool;
+    }.
+
+  Definition send_obs (id: fin' n) (msg: T) :=
+    Log {| id := id; sent := Some msg; recd := None; term := false |}.
+
+  Definition recv_obs (id: fin' n) (msg: T) :=
+    Log {| id := id; sent := None; recd := Some msg; term := false |}.
+
+  Definition empty_obs (id: fin' n) :=
+    Log {| id := id; sent := None; recd := None; term := false |}.
+
+  Definition term_obs (id: fin' n) :=
+    Log {| id := id; sent := None; recd := None; term := true |}.
+
+  (* A distributed system is a vector of workers *)
+  Notation Sys := (vec' n Worker).
+  
+  Definition upd_mbox(sys: Sys)(id: fin' n)(m: option T) :=
+    sys @ id := {| mbox := m; proc := proc (sys $ id) |}.
+
+  Definition upd_proc(sys: Sys)(id: fin' n)(p: ctree netE unit) :=
+    sys @ id := {| mbox := mbox (sys $ id); proc := p |}.
+
+  Equations uring_sched_one' (id: fin' n)(sys: Sys): ctree (writerE NetObs) (fin' n * Sys) :=
+    uring_sched_one' id sys with observe_worker (sys $ id) => {
+        (** A non-deterministic choice, traverse it *)
+        uring_sched_one' _ _ (mbox, BrF n' k) :=
+          Br n' (fun i => Ret (id, upd_proc sys id (k i)));
+        
+        (** A guard, traverse it *)
+        uring_sched_one' _ _ (mbox, GuardF t') :=
+          Guard (Ret (id, upd_proc sys id t'));
+        
+        (** A network `send` effect, interpet it and context-switch right*)
+        uring_sched_one' _ _ (mbox, VisF (Send m) k) :=
+          Vis (send_obs id m)
+            (fun _ => Ret (cycle id,                       
+                       (upd_mbox
+                          (upd_proc sys id (k tt))
+                          (cycle id) (Some m))));
+          
+        (** Receive a message, full mailbox *)
+        uring_sched_one' _ _ (Some m, VisF Recv k) :=
+          Vis (recv_obs id m)
+            (fun _ => Ret (id,
+                       (upd_mbox
+                          (upd_proc sys id (k None))
+                          id None)));
+
+        (** Receive a message, empty mailbox *)
+        uring_sched_one' _ _ (None, VisF Recv k) :=
+          Vis (empty_obs id) (fun _ => Ret (id, upd_proc sys id (k None)));
+
+        (** A process returns, mark it as complete *)
+        uring_sched_one' _ _ (_, RetF tt) :=
+          Vis (term_obs id) (fun _ => Ret (cycle id, upd_proc sys id Ctree.stuck));
+      }.
+
+  (* Nondeterministic pick which process to start first,
+     then schedule processes in a unidirectional ring *)
+  Definition uring_sched (sys: Sys): ctree (writerE NetObs) void :=
+    id <- Ctree.branch n;;
+    Ctree.forever void
+      (fun '(id, sys) =>  uring_sched_one' id sys) (id, sys).
+
+End UniringMsg.
